\documentclass[11pt, oneside]{article}   	% use "amsart" instead of "article" for AMSLaTeX format
\usepackage{geometry}                		% See geometry.pdf to learn the layout options. There are lots.
\geometry{letterpaper}                   		% ... or a4paper or a5paper or ... 
%\geometry{landscape}                		% Activate for rotated page geometry
\usepackage[parfill]{parskip}    			% Activate to begin paragraphs with an empty line rather than an indent
\usepackage{graphicx}				% Use pdf, png, jpg, or epsÂ§ with pdflatex; use eps in DVI mode
								% TeX will automatically convert eps --> pdf in pdflatex		
\usepackage{amssymb}
\usepackage{amsmath, amsfonts}
\usepackage{mathtools}
\usepackage{enumerate}
\usepackage{tikz}

\usetikzlibrary{arrows}

\def\firstcircle{(90:1.75cm) circle (2.5cm)}
\def\secondcircle{(210:1.75cm) circle (2.5cm)}
\def\thirdcircle{(330:1.75cm) circle (2.5cm)}


%SetFonts

%SetFonts


\title{\bf MATH 180 - Homework 4}
\author{Lixiao Yang - \texttt{ly364@drexel.edu}}
\date{February 7, 2023}							% Activate to display a given date or no date

\begin{document}

\maketitle

\section*{Question 1}

	\subsection*{Part a}
	$\because$ Each term differs from the $n^{th}$ power of 2 by 3.\\
	$\therefore a_{n}=2^{n}+3$

	\subsection*{Part b}
	$\because$ Each number is one less than the integer square.\\
	$\therefore a_{n}=(n+1)^{2}-1$

	\subsection*{Part c}
	$\because$ Each element is the product of two adjacent numbers.\\
	$\therefore a_{n}=(n+2)(n+3)=n^{2}+5n+6$.

	\subsection*{Part d}
	$\because$ The difference between each two items is increased by 3 each time.\\
	$\therefore a_{n}=\frac{n(3n+1)}{2}$

\section*{Question 2}

	$a_{0}=0, a_{1}=1, a_{2}=3, a_{3}=7, a_{4}=15, a_{5}=31$\\
	Closed formula: $a_{n}=2^{n}-1$

\section*{Question 3}

	$a_{0}=0, a_{1}=2, a_{2}=6, a_{3}=12, a_{4}=20, a_{5}=30$\\
	Recursive formula: $a_{n}=a_{n-1}+2n$ with $a_{0}=0$

\section*{Question 4}

	$7a_{n-1}-10a_{n-2}$\\
	$=7(2^{n-1}+5^{n-1})-10(2^{n-2}+5^{n-2})$\\
	$=4\cdot 2^{n-2}-25\cdot 5^{n-2}$\\
	$=2^{n}-5^{n}=a_{n}$\\
	$\therefore$ The initial conditions are $a_{0}=0$ and $a_{1}=-3$.

\section*{Question 5}

	$(2+59)\times 10=610$


\section*{Question 6}

	$\frac{(77-3)\times 21}{2}=777$

\section*{Question 7}

	$\because a_{0}=1$\\
	$\therefore S_{n}=n+2n(n+1)+1=2n^{2}+3n+1$

\section*{Question 8}

	$S-2S=-S=3-3\cdot 2^{n+1}$\\
	$S_{n}=3\cdot 2^{n+1}-3$

\section*{Question 9}

	Let $N=0.\overline{37}$\\
	$\because 0.99N=0.37$\\
	$\therefore 0.\overline{37}=\frac{37}{99}$

\section*{Question 10}

	Let $N=0.\overline{213}$\\
	$\because 0.999N=0.213$\\
	$\therefore 0.\overline{213}=\frac{213}{999}$

\end{document}  